\url{http://www.mathhelpforum.com/math-help/calculus/63-line-tangent-elipse-given-one-point.html}

Posted 13 April 2005

\paragraph{Question} Write the equations of the tangent lines from $\left(3,0\right)$ to

\begin{equation}
	x^2+2y^2=6.\label{63a}
\end{equation}

\paragraph{Solution} \solutionAuthor{ticbol}

The slope of the tangent line is $\frac{dy}{dx}$. Thus, to find $\frac{dy}{dx}$, we differentiate $x^2+2y^2=6$ implicitly with respect to $x$.

\begin{eqnarray*}
	\frac{d}{dx}\left(x^2+2y^2\right)&=&\frac{d}{dx}\left(6\right)\\
	\Rightarrow dx+2y\frac{dy}{dx}&=&0\\
	\Rightarrow 4\frac{dy}{dx}&=&-2x\\
	\Rightarrow \frac{dy}{dx}&=&-\frac{2x}{4y}\\
	&=&-\frac{x}{2y}
\end{eqnarray*}

Let $\left(x,y\right)$ be the point at which the tangent line touches the ellipse.

We have two points on the tangent line, $\left(3,0\right)$ and $\left(x,y\right)$.

We can determine the slope $m$ of the tangent line from these two points:

\begin{eqnarray*}
	m&=&\frac{y-0}{x-3}\\
	&=&\frac{y}{x-3},
\end{eqnarray*}

which is the same as $\frac{dy}{dx}$.

\begin{eqnarray}
	\therefore-\frac{x}{2y}&=&\frac{y}{x-3}\nonumber\\
	\Rightarrow-x\left(x-3\right)&=&\left(2y\right)y\nonumber\\
	\Rightarrow-x^2+3x=2y^2\label{63b}
\end{eqnarray}

\begin{eqnarray}
	x^2+2y^2&=&6\qquad\mbox{(from \ref{63a})}\nonumber\\
	\Rightarrow2y^2&=&6-x^2\label{63c}
\end{eqnarray}

\begin{eqnarray}
	3x&=&6\qquad\mbox{(substitute \ref{63c} into \ref{63b})}\nonumber\\
	\Rightarrow x&=&\frac{6}{3}\label{63d}\\
	&=&2\nonumber
\end{eqnarray}

\begin{eqnarray*}
	2^2+2y^2&=&6\qquad\mbox{(substitute \ref{63d} into \ref{63a})}\\
	\Rightarrow2y^2&=&6-2^2\\
	&=&2\\
	\Rightarrow y^2&=&\frac{2}{2}\\
	&=&1\\
	\Rightarrow y&=&\pm\sqrt{1}.
\end{eqnarray*}

This means that there are two points at which the tangent line touches the ellipse.
